AVM/Class/Translation/Logics.lean
@@ -1,0 +1,84 @@
+import AVM.Class
+import AVM.Message
+import AVM.Logic
+
+namespace AVM.Class
+
+/-- Creates a message logic for a given constructor. -/
+def Constructor.Message.logic
+  {lab : Ecosystem.Label}
+  {classId : lab.ClassId}
+  {constrId : classId.label.ConstructorId}
+  (constr : Class.Constructor classId constrId)
+  (args : Logic.Args)
+  : Bool :=
+  let try msg : Message classId.label := Message.fromResource args.self
+  let try argsData := SomeType.cast msg.args
+  let try vals : (constr.body argsData).params.Product := tryCast msg.vals
+  let newObjData := constr.body argsData |>.value vals
+  let consumedResObjs := Logic.selectObjectResources args.consumed
+  let createdResObjs := Logic.selectObjectResources args.created
+  Logic.checkResourcesData [newObjData.toSomeObjectData] consumedResObjs
+    && Logic.checkResourcesData [newObjData.toSomeObjectData] createdResObjs
+    && Logic.checkResourcesEphemeral consumedResObjs
+    && Logic.checkResourcesPersistent createdResObjs
+    && constr.invariant argsData
+
+/-- Creates a message logic for a given destructor. -/
+def Destructor.Message.logic
+  {lab : Ecosystem.Label}
+  {classId : lab.ClassId}
+  {destructorId : classId.label.DestructorId}
+  (destructor : Class.Destructor classId destructorId)
+  (args : Logic.Args)
+  : Bool :=
+  let try msg : Message classId.label := Message.fromResource args.self
+  let try argsData := SomeType.cast msg.args
+  let consumedResObjs := Logic.selectObjectResources args.consumed
+  let createdResObjs := Logic.selectObjectResources args.created
+  let! [selfRes] := consumedResObjs
+  let try selfObj : Object classId.label := Object.fromResource selfRes
+  Logic.checkResourcesData [selfObj.toSomeObjectData] createdResObjs
+    && Logic.checkResourcesPersistent consumedResObjs
+    && Logic.checkResourcesEphemeral createdResObjs
+    && destructor.invariant selfObj argsData
+
+/-- Creates a message logic for a given method. -/
+def Method.Message.logic
+  {lab : Ecosystem.Label}
+  {classId : lab.ClassId}
+  {methodId : classId.label.MethodId}
+  (method : Class.Method classId methodId)
+  (args : Logic.Args)
+  : Bool :=
+  let try msg : Message classId.label := Message.fromResource args.self
+  let try argsData := SomeType.cast msg.args
+  let consumedResObjs := Logic.selectObjectResources args.consumed
+  let createdResObjs := Logic.selectObjectResources args.created
+  let! [selfRes] := consumedResObjs
+  let try selfObj : Object classId.label := Object.fromResource selfRes
+  check method.invariant selfObj argsData
+  let body := method.body selfObj argsData
+  let try vals : body.params.Product := tryCast msg.vals
+  let createdObject : Object classId.label := body |>.value vals
+  Logic.checkResourcesData [createdObject.toSomeObjectData] createdResObjs
+    && Logic.checkResourcesPersistent consumedResObjs
+    && Logic.checkResourcesPersistent createdResObjs
+
+/-- The class logic checks if all consumed messages in the action correspond
+  to class members and the single consumed object is the receiver. -/
+def logic {lab : Ecosystem.Label} {classId : lab.ClassId} (cl : Class classId) (args : Logic.Args) : Bool :=
+  let try self : Object classId.label := Object.fromResource args.self
+  check cl.invariant self args
+  match args.status with
+  | Created => true
+  | Consumed =>
+    let consumedMessageResources : List Anoma.Resource := Logic.selectMessageResources args.consumed
+    let! [consumedObjectResource] : List Anoma.Resource := Logic.selectObjectResources args.consumed
+    let try consumedObject : Object classId.label := Object.fromResource consumedObjectResource
+    consumedMessageResources.length + 1 == (Logic.filterOutDummy args.consumed).length
+      && consumedMessageResources.all fun res =>
+        let try msg : Message classId.label := Message.fromResource res
+        -- NOTE: we should check that the resource logic of res corresponds to
+        -- the message logic
+        consumedObject.uid == msg.recipient
