AVM/Class/Translation/Tasks.lean
@@ -1,0 +1,195 @@
+import Mathlib.Control.Random
+import Anoma
+import AVM.Tasks
+import AVM.Ecosystem
+import AVM.Class.Translation.Messages
+
+namespace AVM.Class
+
+/-- Type of functions which adjust object values by modifications that occurred
+  in the program up to a certain point. -/
+abbrev AdjustFun := {clab : Class.Label} → Object clab → Object clab
+
+private structure Task' where
+  task : Task
+  /-- Function which adjusts object values by modifications that occurred in the
+    program up to the point after the task, i.e., up to and including the part
+    of the program corresponding to the task. -/
+  adjust : task.params.Product → AdjustFun
+  deriving Inhabited
+
+/-- A helper type for data at the end of `Tasks` execution. -/
+private structure TasksResult (params : Program.Parameters) (α : Type u) where
+  /-- The return value of the tasks. -/
+  value : α
+  /-- Function which adjusts object values by modifications that occurred in the
+    program up to after the tasks, i.e., up to and including the part of the
+    program corresponding to the tasks. -/
+  adjust : AdjustFun
+  /-- Body parameter values adjusted by preceding modifications in the program. -/
+  bodyParameterValues : params.Product
+  deriving Inhabited
+
+mutual
+
+/-- Creates `Tasks` for a given `body` program. The `adjust` argument adjusts
+   object values by modifications that occurred in the program up to before
+   executing `body`. The result in `TasksResult` contains:
+ 1. The return value of the body.
+ 2. The `adjust` function which adjusts object values by modifications that
+    occurred in the program up to after executing `body`.
+ 3. The adjusted values of body parameters (adjusted values in
+    `body.params.Product`). -/
+private partial def Body.tasks'
+  (adjust : AdjustFun)
+  {α}
+  [Inhabited α]
+  {lab : Ecosystem.Label}
+  (eco : Ecosystem lab)
+  (body : Program lab α)
+  : Tasks (TasksResult body.params α) :=
+  match body with
+  | .constructor classId constrId args next =>
+    let constr := eco.classes classId |>.constructors constrId
+    Tasks.rand fun newId => Tasks.rand fun r =>
+      let task := constr.task' adjust eco newId r args
+      Tasks.task task.task fun vals =>
+        Body.tasks' (task.adjust vals) eco (next newId)
+        |>.map (fun res => ⟨res.value, res.adjust, ⟨newId, res.bodyParameterValues⟩⟩)
+  | .destructor classId destrId selfId args next =>
+    let destr := eco.classes classId |>.destructors destrId
+    Tasks.fetch ⟨classId.label, selfId⟩ fun self => Tasks.rand fun r =>
+      let task := destr.task' adjust eco r (adjust self) args
+      Tasks.task task.task fun vals =>
+        Body.tasks' (task.adjust vals) eco next
+  | .method classId methodId selfId args next =>
+    let method := eco.classes classId |>.methods methodId
+    Tasks.fetch ⟨classId.label, selfId⟩ fun self => Tasks.rand fun r =>
+      let task := method.task' adjust eco r (adjust self) args
+      Tasks.task task.task fun vals =>
+        Body.tasks' (task.adjust vals) eco next
+  | .fetch objId next =>
+    Tasks.fetch objId fun obj =>
+      Body.tasks' adjust eco (next (adjust obj))
+      |>.map (fun res => ⟨res.value, res.adjust, ⟨adjust obj, res.bodyParameterValues⟩⟩)
+  | .return val =>
+    Tasks.result ⟨val, adjust, ()⟩
+
+private partial def Member.task'
+  {α}
+  [Inhabited α]
+  (adjust : AdjustFun)
+  {lab : Ecosystem.Label}
+  (eco : Ecosystem lab)
+  (body : Program lab α)
+  (mkActionData : α → List SomeConsumableObject × List CreatedObject)
+  (mkMessage : body.params.Product → SomeMessage)
+  : Task' :=
+  let tasks : Tasks (TasksResult body.params α) :=
+    Body.tasks' adjust eco body
+  let task :=
+    Tasks.composeWithMessage
+      tasks
+      (fun res => mkMessage res.bodyParameterValues)
+      (mkActionData ∘ TasksResult.value)
+  let mkAdjust (vals : task.params.Product) : AdjustFun :=
+    let res := tasks.value (Tasks.coerce vals)
+    let (_, createdObjects) := mkActionData res.value
+    let adjust' : AdjustFun := fun obj =>
+      let try createdObj := createdObjects.find? (fun o => o.uid == obj.uid)
+          failwith obj
+      let try obj' := tryCast createdObj.toObject
+          failwith obj
+      obj'
+    adjust' ∘ res.adjust
+  ⟨task, mkAdjust⟩
+
+/-- Creates a Task for a given object constructor. -/
+private partial def Constructor.task'
+  (adjust : AdjustFun)
+  {lab : Ecosystem.Label}
+  (eco : Ecosystem lab)
+  {classId : lab.ClassId}
+  {constrId : classId.label.ConstructorId}
+  (constr : Class.Constructor classId constrId)
+  (newId : ObjectId)
+  (r : Nat)
+  (args : constrId.Args.type)
+  : Task' :=
+  let body : Program lab (ObjectData classId.label) := constr.body args
+  let mkActionData (newObjectData : ObjectData classId.label) : List SomeConsumableObject × List CreatedObject :=
+    let newObj : SomeObject :=
+      let obj : Object classId.label :=
+        { uid := newId,
+          nonce := ⟨newId⟩,
+          data := newObjectData }
+      obj.toSomeObject
+    let consumedObj := newObj.toConsumable (ephemeral := true)
+    let createdObjects : List CreatedObject :=
+      [CreatedObject.fromSomeObject newObj (ephemeral := false) (rand := r)]
+    ([consumedObj], createdObjects)
+  let mkMessage (vals : body.params.Product) : SomeMessage :=
+    constr.message ⟨body.params.Product⟩ vals newId args
+  Member.task' adjust eco body mkActionData mkMessage
+
+/-- Creates a Task for a given object destructor. -/
+private partial def Destructor.task'
+  (adjust : AdjustFun)
+  {lab : Ecosystem.Label}
+  (eco : Ecosystem lab)
+  {classId : lab.ClassId}
+  {destructorId : classId.label.DestructorId}
+  (destructor : Class.Destructor classId destructorId)
+  (r : Nat)
+  (self : Object classId.label)
+  (args : destructorId.Args.type)
+  : Task' :=
+  let body : Program lab Unit := destructor.body self args
+  let mkActionData (_ : Unit) : List SomeConsumableObject × List CreatedObject :=
+    let consumedObj := self.toSomeObject.toConsumable (ephemeral := false)
+    let createdObjects : List CreatedObject :=
+      [{ uid := self.uid,
+         data := self.data,
+         ephemeral := true,
+         rand := r }]
+    ([consumedObj], createdObjects)
+  let mkMessage (vals : body.params.Product) : SomeMessage :=
+    destructor.message ⟨body.params.Product⟩ vals self.uid args
+  Member.task' adjust eco body mkActionData mkMessage
+
+/-- Creates a Task for a given method. -/
+private partial def Method.task'
+  (adjust : AdjustFun)
+  {lab : Ecosystem.Label}
+  (eco : Ecosystem lab)
+  {classId : lab.ClassId}
+  {methodId : classId.label.MethodId}
+  (method : Class.Method classId methodId)
+  (r : Nat)
+  (self : Object classId.label)
+  (args : methodId.Args.type)
+  : Task' :=
+  let body : Program lab (Object classId.label) := method.body self args
+  let mkActionData (obj : Object classId.label) : List SomeConsumableObject × List CreatedObject :=
+    let consumedObj := self.toSomeObject.toConsumable (ephemeral := false)
+    let createdObjects : List CreatedObject :=
+      [{ uid := obj.uid,
+         data := obj.data,
+         ephemeral := false,
+         rand := r }]
+    ([consumedObj], createdObjects)
+  let mkMessage (vals : body.params.Product) : SomeMessage :=
+    method.message ⟨body.params.Product⟩ vals self.uid args
+  Member.task' adjust eco body mkActionData mkMessage
+
+end -- mutual
+
+/-- Creates Tasks for a given class member body program. -/
+def Member.Body.tasks
+  {α}
+  [Inhabited α]
+  {lab : Ecosystem.Label}
+  (eco : Ecosystem lab)
+  (prog : Program lab α)
+  : Tasks α :=
+  Body.tasks' id eco prog |>.map TasksResult.value
