AVM/Program/Parameters.lean
@@ -2,24 +2,63 @@ import AVM.Object
 
 namespace AVM
 
+/-- Type describing the parameters of a program. Program parameters are the
+  random values generated and the objects fetched inside the program. -/
 inductive Program.Parameters where
   | empty
   | fetch (param : TypedObjectId) (rest : Object param.classLabel → Program.Parameters)
-  | genId (rest : ObjectId → Program.Parameters)
+  | rand (rest : Nat → Program.Parameters)
 deriving Inhabited, Nonempty
 
+/-- Generate a random unique ObjectId. -/
+def Program.Parameters.genId (rest : ObjectId → Program.Parameters) : Program.Parameters :=
+  .rand rest
+
+/-- Type of program parameter values. Program parameter values can be adjusted
+  or unadjusted. Unadjusted parameter values are the values of parameters at the
+  start of the program, before any of the program instructions are executed
+  (this makes a difference only for object values). Adjusted parameter values
+  are the values of parameters at the point in the program where they are
+  fetched. For example, in the following program the adjusted value of `obj` is
+  equal to the unadjusted value of `obj` with `obj.count` incremented by `n`:
+  ```
+  example (objId : ObjectId) (n : Nat) : Program lab Nat :=
+    Program.method Counter Counter.Increment objId n <|
+    Program.fetch ⟨Counter, objId⟩ fun obj =>
+      Program.return obj.count
+  ```
+-/
 def Program.Parameters.Product (params : Program.Parameters) : Type u :=
   match params with
   | .empty => PUnit
   | .fetch param rest =>
     Σ (obj : Object param.classLabel), Program.Parameters.Product (rest obj)
-  | .genId rest =>
-    Σ (objId : ObjectId), Program.Parameters.Product (rest objId)
+  | .rand rest =>
+    Σ (r : Nat), Program.Parameters.Product (rest r)
+
+private def Program.Parameters.Product.defaultValue (params : Program.Parameters) : params.Product :=
+  match params with
+  | .empty => PUnit.unit
+  | .fetch _ rest =>
+    ⟨default, Product.defaultValue (rest default)⟩
+  | .rand rest =>
+    ⟨default, Product.defaultValue (rest default)⟩
+
+instance {params : Program.Parameters} : Inhabited params.Product where
+  default := Program.Parameters.Product.defaultValue params
 
 instance {params : Program.Parameters} : TypeRep params.Product where
   rep := Rep.atomic "Program.Parameters.Product" -- TODO: this should depend on params
 
 namespace Program.Parameters
+
+def map (f : {lab : Class.Label} → Object lab → Object lab) (params : Program.Parameters) : Program.Parameters :=
+  match params with
+  | .empty => .empty
+  | .fetch p rest =>
+    .fetch p (fun obj => map f (rest (f obj)))
+  | .rand rest =>
+    .rand (fun r => map f (rest r))
 
 def Product.beq {params : Program.Parameters} (a b : params.Product) :=
     match params with
@@ -30,10 +69,10 @@ def Product.beq {params : Program.Parameters} (a b : params.Product) :=
       check objA == objB
       let try valsB' := tryCast valsB
       beq valsA valsB'
-    | .genId _ =>
-      let ⟨objIdA, valsA⟩ := a
-      let ⟨objIdB, valsB⟩ := b
-      check objIdA == objIdB
+    | .rand _ =>
+      let ⟨rA, valsA⟩ := a
+      let ⟨rB, valsB⟩ := b
+      check rA == rB
       let try valsB' := tryCast valsB
       beq valsA valsB'
 
@@ -47,16 +86,25 @@ def append (params1 : Program.Parameters) (params2 : params1.Product → Program
   | .fetch p1 ps1 =>
     .fetch p1
       (fun obj => (ps1 obj).append (fun vals => params2 ⟨obj, vals⟩))
-  | .genId ps1 =>
-    .genId (fun objId => (ps1 objId).append (fun vals => params2 ⟨objId, vals⟩))
+  | .rand ps1 =>
+    .rand (fun r => (ps1 r).append (fun vals => params2 ⟨r, vals⟩))
 
-def concat (params : List Program.Parameters) : Program.Parameters :=
-  match params with
-  | [] => .empty
-  | ps :: rest =>
-    ps.append (fun _ => concat rest)
+def Product.append
+  {params1 : Program.Parameters}
+  {params2 : params1.Product → Program.Parameters}
+  (vals1 : params1.Product)
+  (vals2 : (params2 vals1).Product)
+  : (params1.append params2).Product :=
+  match params1 with
+  | .empty => vals2
+  | .fetch _ _ =>
+    let ⟨obj, vals1'⟩ := vals1
+    ⟨obj, Product.append vals1' vals2⟩
+  | .rand _ =>
+    let ⟨r, vals1'⟩ := vals1
+    ⟨r, Product.append vals1' vals2⟩
 
-def splitProduct
+def Product.split
   {params1 : Program.Parameters}
   {params2 : params1.Product → Program.Parameters}
   (vals : params1.append params2 |>.Product)
@@ -65,20 +113,9 @@ def splitProduct
   | .empty => ⟨PUnit.unit, vals⟩
   | .fetch _ _ =>
     let ⟨obj, vals'⟩ := vals
-    let ⟨vals1, vals2⟩ := splitProduct vals'
+    let ⟨vals1, vals2⟩ := vals'.split
     ⟨⟨obj, vals1⟩, vals2⟩
-  | .genId _ =>
-    let ⟨objId, vals'⟩ := vals
-    let ⟨vals1, vals2⟩ := splitProduct vals'
-    ⟨⟨objId, vals1⟩, vals2⟩
-
-def splitProducts
-  {params : List Program.Parameters}
-  (vals : Program.Parameters.concat params |>.Product)
-  : HList (params.map Program.Parameters.Product) :=
-  match params with
-  | [] => HList.nil
-  | _ :: ps =>
-    let ⟨vals1, vals'⟩ := splitProduct vals
-    let rest : HList (ps.map Program.Parameters.Product) := splitProducts vals'
-    HList.cons vals1 rest
+  | .rand _ =>
+    let ⟨r, vals'⟩ := vals
+    let ⟨vals1, vals2⟩ := vals'.split
+    ⟨⟨r, vals1⟩, vals2⟩
