AVM/Task.lean
@@ -16,8 +16,9 @@ structure Task.Actions where
   level of abstraction to compose translations of different message sends,
   enabling nested method calls and subobjects. -/
 structure Task.{u} : Type (u + 1) where
-  /-- Task parameters - objects to fetch from the Anoma system and new object
-    ids to generate. -/
+  /-- Task parameters - objects to fetch from the Anoma system and random values
+    to generate. In general, values in `task.params.Product` are assumed to be
+    unadjusted (see `Program.Parameters.Product`). -/
   params : Program.Parameters
   /-- The message to send to the recipient. -/
   message : params.Product → Option SomeMessage
@@ -29,75 +30,18 @@ deriving Inhabited
 def Task.absorbParams.{u} (params : Program.Parameters) (task : params.Product → Task.{u}) : Task.{u} :=
   { params := params.append (fun vals => (task vals).params),
     message := fun vals =>
-      let ⟨vals1, vals2⟩ := Program.Parameters.splitProduct vals
+      let ⟨vals1, vals2⟩ := vals.split
       (task vals1).message vals2,
     actions := fun vals =>
-      let ⟨vals1, vals2⟩ := Program.Parameters.splitProduct vals
+      let ⟨vals1, vals2⟩ := vals.split
       (task vals1).actions vals2 }
 
-def Task.Products (tasks : List Task) : List Type :=
-  tasks.map (·.params) |> .map (·.Product)
+def Task.absorbGenId (task : ObjectId → Task) : Task :=
+  Task.absorbParams
+    (Program.Parameters.genId (fun _ => .empty))
+    (fun ⟨newId, ()⟩ => task newId)
 
-def Task.makeActions
-  (tasks : List Task)
-  (vals : HList (Products tasks))
-  : Rand (Option Task.Actions) :=
-  match tasks, vals with
-  | [], _ => pure <| some { actions := [], deltaWitness := Anoma.DeltaWitness.empty }
-  | task :: tasks', HList.cons vals' vals'' => do
-    let try actions ← task.actions vals'
-    let try rest ← makeActions tasks' vals''
-    pure <| some <|
-      { actions := actions.actions ++ rest.actions,
-        deltaWitness := Anoma.DeltaWitness.compose actions.deltaWitness rest.deltaWitness }
-
-def Task.composeMessages (tasks : List Task) (vals : HList (Products tasks)) : List SomeMessage :=
-  match tasks, vals with
-  | [], _ => []
-  | task :: tasks', HList.cons vals' vals'' =>
-    (task.message vals' |>.toList) ++
-      composeMessages tasks' vals''
-
-def Task.composeParams (tasks : List Task) : Program.Parameters :=
-  tasks |>.map (·.params) |> .concat
-
-def Task.composeActions
-  (tasks : List Task)
-  (mkAction : HList (Products tasks) → Rand (Option (Anoma.Action × Anoma.DeltaWitness)))
-  (vals : (Task.composeParams tasks).Product)
-  : Rand (Option Task.Actions) := do
-  let vals' := Program.Parameters.splitProducts vals
-  let try actions ← Task.makeActions tasks vals'
-  let try (action, witness) ← mkAction vals'
-  pure <| some <|
-    { actions := action :: actions.actions,
-      deltaWitness := Anoma.DeltaWitness.compose witness actions.deltaWitness }
-
-def Task.composeWithAction
-  (msg : Option SomeMessage)
-  (tasks : List Task)
-  (mkAction : HList (Products tasks) → Rand (Option (Anoma.Action × Anoma.DeltaWitness)))
-  : Task :=
-  { params := composeParams tasks,
-    message := fun _ => msg,
-    actions := composeActions tasks mkAction }
-
-def Task.composeWithMessage
-  (msg : SomeMessage)
-  (tasks : List Task)
-  (consumedObjs : List SomeConsumableObject)
-  (createdObjects : List CreatedObject)
-  : Task :=
-  let mkAction (vals : HList (Products tasks))
-    : Rand (Option (Anoma.Action × Anoma.DeltaWitness)) :=
-    let try consumedObjects := consumedObjs.map (·.consume) |>.getSome
-    let createdMessages := composeMessages tasks vals
-    Action.create consumedObjects createdObjects [msg] createdMessages
-  Task.composeWithAction msg tasks mkAction
-
-def Task.compose (tasks : List Task) : Task :=
-  let mkAction (vals : HList (Products tasks))
-    : Rand (Option (Anoma.Action × Anoma.DeltaWitness)) :=
-    let createdMessages := composeMessages tasks vals
-    Action.create [] [] [] createdMessages
-  Task.composeWithAction none tasks mkAction
+def Task.absorbFetch (param : TypedObjectId) (task : Object param.classLabel → Task) : Task :=
+  Task.absorbParams
+    (Program.Parameters.fetch param (fun _ => .empty))
+    (fun ⟨obj, ()⟩ => task obj)
