AVM/Tasks.lean
@@ -1,0 +1,140 @@
+import AVM.Task
+
+namespace AVM
+
+/-- The `Tasks` type represents a sequence of tasks with intervening object
+  fetches and random value generations. The `Tasks` type mimics more closely the
+  structure of AVM programs than a single `Task`. `AVM.Program` is compiled to
+  `Tasks` which are then composed into a single `Task`. The composition of
+  `Tasks` collects and lifts out the parameters of all subtasks. -/
+inductive Tasks (α : Type u) where
+  /-- Execute a subtask and continue. The `rest` continuation receives the
+    unadjusted parameter values. -/
+  | task (task : Task) (rest : task.params.Product → Tasks α) : Tasks α
+  /-- Fetch an object and continue. The `rest` continuation receives the
+    unadjusted original object value and is supposed to adjust it by the
+    modifications to that object that occurred from the start of the program up
+    to the fetch. -/
+  | fetch (param : TypedObjectId) (rest : Object param.classLabel → Tasks α) : Tasks α
+  | rand (rest : Nat → Tasks α) : Tasks α
+  | result (value : α) : Tasks α
+  deriving Inhabited
+
+/-- `Tasks.params` includes the parameters of the sub-tasks, in contrast to
+  `Program.params` which doesn't include the parameters of the sub-programs. In
+  general, values in `tasks.params.Product` are assumed to be unadjusted (see
+  `Program.Parameters.Product`), in contrast to values in `prog.params.Product`
+  which are assumed to be adjusted. -/
+def Tasks.params {α} (tasks : Tasks α) : Program.Parameters :=
+  match tasks with
+  | .task t rest => (t.params.append (fun vals => (rest vals).params))
+  | .fetch p rest => .fetch p (fun obj => (rest obj).params)
+  | .rand rest => .rand (fun r => (rest r).params)
+  | .result _ => .empty
+
+/-- The return value of the tasks. `vals` are unadjusted parameter values (see
+  `Program.Parameters.Product`): the object values as fetched from Anoma at the
+  start of program execution, i.e., they are not adjusted by subsequent
+  modifications to these objects in the program. -/
+def Tasks.value {α} (tasks : Tasks α) (vals : tasks.params.Product) : α :=
+  match tasks with
+  | .task _ rest =>
+    let ⟨vals1, vals2⟩ := vals.split
+    Tasks.value (rest vals1) vals2
+  | .fetch _ rest =>
+    let ⟨obj, vals'⟩ := vals
+    Tasks.value (rest obj) vals'
+  | .rand rest =>
+    let ⟨r, vals'⟩ := vals
+    Tasks.value (rest r) vals'
+  | .result v => v
+
+def Tasks.map' {α β} (tasks : Tasks α) (f : tasks.params.Product → α → β) : Tasks β :=
+  match tasks with
+  | .task t rest => .task t (fun vals => map' (rest vals) (fun vals' => f (vals.append vals')))
+  | .fetch p rest => .fetch p (fun obj => map' (rest obj) (fun vals' => f ⟨obj, vals'⟩))
+  | .rand rest => .rand (fun r => map' (rest r) (fun vals' => f ⟨r, vals'⟩))
+  | .result v => .result (f () v)
+
+def Tasks.map {α β} (tasks : Tasks α) (f : α → β) : Tasks β :=
+  tasks.map' (fun _ a => f a)
+
+def Tasks.coerce {α β} {tasks : Tasks α} {f : tasks.params.Product → α → β} (vals : (tasks.map' f).params.Product) : tasks.params.Product :=
+  match tasks with
+  | .task _ _ =>
+    let ⟨vals1, vals2⟩ := vals.split
+    vals1.append (coerce vals2)
+  | .fetch _ _ =>
+    let ⟨obj, vals'⟩ := vals
+    ⟨obj, coerce vals'⟩
+  | .rand _ =>
+    let ⟨r, vals'⟩ := vals
+    ⟨r, coerce vals'⟩
+  | .result _ => vals
+
+def TasksWithAction := Tasks (Rand (Option (Anoma.Action × Anoma.DeltaWitness)))
+
+def Tasks.composeActions
+  (tasks : TasksWithAction)
+  (vals : tasks.params.Product)
+  : Rand (Option Task.Actions) :=
+  match tasks with
+  | .result v => do
+    let try (action, witness) ← v
+    pure <| some { actions := [action], deltaWitness := witness }
+  | .task ta rest => do
+    let ⟨vals1, vals2⟩ := vals.split
+    let try actions ← ta.actions vals1
+    let try rest' ← composeActions (rest vals1) vals2
+    pure <| some <|
+      { actions := actions.actions ++ rest'.actions,
+        deltaWitness := Anoma.DeltaWitness.compose actions.deltaWitness rest'.deltaWitness }
+  | .fetch _ rest =>
+    let ⟨obj, vals'⟩ := vals
+    composeActions (rest obj) vals'
+  | .rand rest =>
+    let ⟨r, vals'⟩ := vals
+    composeActions (rest r) vals'
+
+def Tasks.composeMessages {α} (tasks : Tasks α) (vals : tasks.params.Product) : List SomeMessage :=
+  match tasks with
+  | .result _ => []
+  | .task ta tasks' =>
+    let ⟨vals1, vals2⟩ := vals.split
+    (ta.message vals1 |>.toList) ++
+      composeMessages (tasks' vals1) vals2
+  | .fetch _ rest =>
+    let ⟨obj, vals'⟩ := vals
+    composeMessages (rest obj) vals'
+  | .rand rest =>
+    let ⟨r, vals'⟩ := vals
+    composeMessages (rest r) vals'
+
+def Tasks.composeWithAction
+  (tasks : TasksWithAction)
+  (msg : tasks.params.Product → Option SomeMessage)
+  : Task :=
+  { params := tasks.params,
+    message := msg,
+    actions := composeActions tasks }
+
+def Tasks.composeWithMessage
+  {α}
+  (tasks : Tasks α)
+  (msg : α → SomeMessage)
+  (objects : α → List SomeConsumableObject × List CreatedObject)
+  : Task :=
+  let mkAction (vals : tasks.params.Product) (a : α)
+    : Rand (Option (Anoma.Action × Anoma.DeltaWitness)) :=
+    let (consumedObjs, createdObjects) := objects a
+    let try consumedObjects := consumedObjs.map (·.consume) |>.getSome
+    let createdMessages := composeMessages tasks vals
+    Action.create consumedObjects createdObjects [msg a] createdMessages
+  Tasks.composeWithAction (tasks.map' mkAction) (fun vals => some (msg (tasks.value (coerce vals))))
+
+def Tasks.compose (tasks : Tasks Unit) : Task :=
+  let mkAction (vals : tasks.params.Product) (_ : Unit)
+    : Rand (Option (Anoma.Action × Anoma.DeltaWitness)) :=
+    let createdMessages := tasks.composeMessages vals
+    Action.create [] [] [] createdMessages
+  Tasks.composeWithAction (tasks.map' mkAction) (fun _ => none)
